DBCircuits.v
@@ -1,0 +1,344 @@
+Require Import Contexts.
+Require Import HOASCircuits.
+Require Import Program.
+Require Import List.
+Require Import Monad.
+Import Arith.
+Open Scope circ_scope.
+
+(* A minimal circuit *)
+(* A well-formed DeBruijn_Circuit n w has exactly n input wires. 
+*)
+Inductive DeBruijn_Circuit (*n : nat*) (w : WType) : Set :=
+| db_output : (*forall {pf : n = size_WType w},*) Pat w -> DeBruijn_Circuit w
+| db_gate   : forall {w1 w2} (*{pf : n + size_WType w2 = n' + size_WType w1}*),
+               Gate w1 w2 -> Pat w1 -> DeBruijn_Circuit w -> DeBruijn_Circuit w
+| db_lift   :  (*{pf : n = S n'}*)
+               Pat Bit -> (bool -> DeBruijn_Circuit w) -> DeBruijn_Circuit w
+.
+
+Inductive DeBruijn_Box (w1 w2 : WType) : Set :=
+| min_box : DeBruijn_Circuit w2 -> DeBruijn_Box w1 w2.
+
+Arguments db_output {w}.
+Arguments db_gate {w w1 w2 }.
+Arguments db_lift {w}.
+
+
+(* Throughout this development, we will want to update some state based on the
+presence of a gate. This is handled by a type class Gate_State, which models how
+a gate might affect some underlying state:
+
+    - We might need to create a fresh variable;
+
+    - We might need to remove a variable from the state;
+
+    - We might need to change the type of a variable in the state. Not all
+      states will keep track of the type, but some will.
+*)
+Class Gate_State A :=
+  { get_fresh  : WType -> State A Var 
+  ; remove_var : Var -> A -> A
+  ; change_type : Var -> WType -> A -> A
+  }.
+
+(* process_gate_pat g p a returns the pattern that is obtained from running the
+   gate g with input pattern p and state a 
+*)
+Definition process_gate_pat {A w1 w2} `{Gate_State A} (g : Gate w1 w2) : Pat w1 -> A -> Pat w2 :=
+  match g with 
+  | U _           => fun p _ => p
+  | init0 | init1 => fun _ a => qubit (fst (get_fresh Qubit a))
+  | new0 | new1   => fun _ a => bit (fst (get_fresh Bit a))
+  | meas          => fun p _ => match p with
+                                | qubit x => bit x
+                                end
+  | discard       => fun _ _ => unit
+  end.
+
+(* process_gate_state g p a returns the state that is obtained from running the
+   gate g with input pattern p and state a. The two functions process_gate_pat
+   and process_gate_state could be combined into one operation in a state monad,
+   but the result requires a lot of bulky infrastructure for dealing with
+   monads, unfortunately. It may be easier just to take two passes over the gate.
+*)
+Definition process_gate_state {A w1 w2} `{Gate_State A} (g : Gate w1 w2) : Pat w1 -> A -> A :=
+  match g with 
+  | U _           => fun _ a => a
+  | init0 | init1 => fun _ a => snd (get_fresh Qubit a)
+  | new0 | new1   => fun _ a => snd (get_fresh Bit a)
+  | meas          => fun p a => match p with
+                                | qubit x => change_type x Bit a
+                                end
+  | discard       => fun p a => match p with
+                                | bit x => remove_var x a
+                                end
+  end.
+
+
+(**********************)  
+(* De Bruijn Contexts *)
+(**********************)
+
+Definition DB_Ctx := list WType.
+Definition DB_to_Ctx (Γ : DB_Ctx) : Ctx := fmap Some Γ.
+
+Fixpoint remove_at  {A} (i : nat) (ls : list A) :=
+  match i, ls with
+  | _   ,[]        => []
+  | 0   , _ :: ls' => ls'
+  | S i', a :: ls' => a :: remove_at i' ls'
+  end.
+Fixpoint update_at {A} (ls : list A) (i : nat) (a : A) : list A :=
+  match ls, i with
+  | []      , _    => []
+  | _ :: ls', 0    => a :: ls'
+  | b :: ls', S i' => b :: update_at ls' i' a
+  end.
+
+
+Instance DB_Ctx_State : Gate_State DB_Ctx :=
+  { get_fresh w  := do Γ ← get;
+                    do _ ← put (w :: Γ);
+                    return_ 0
+  ; remove_var := remove_at
+  ; change_type x w Γ := update_at Γ x w
+  }.
+
+
+(**********)
+(* Typing *)
+(**********)
+
+Definition Types_DB_Pat {w} (Γ : DB_Ctx) (p : Pat w) := Types_Pat (DB_to_Ctx Γ) p.
+
+(* Although we use ordinary (nominal) contexts for typing, it should be the case
+that they are always "minimal", meaning that the list is equivalent to a list of
+WTypes (as opposed to list (option WType)). However, because of context
+splitting, this will only be enforcable at the top level. *)
+Inductive Types_DB {w} (Γ : DB_Ctx) : DeBruijn_Circuit w -> Prop :=
+| types_db_output : forall p, Types_DB_Pat Γ p -> Types_DB Γ (db_output p)
+| types_db_gate   : forall Γ1 Γ2 w1 w2 (g : Gate w1 w2) p c,
+                    Γ = Γ1 ++ Γ2 ->
+                    Types_DB_Pat Γ1 p ->
+                    Types_DB ((process_gate_state g p Γ1) ++ Γ2 ) c ->
+                    Types_DB Γ (db_gate g p c)
+| types_db_lift   : forall Γ1 Γ2 p f,
+                    Γ = Γ1 ++ Γ2 ->
+                    Types_DB_Pat Γ1 p ->
+                    (forall b, Types_DB Γ2 (f b)) ->
+                    Types_DB Γ (db_lift p f)
+.
+
+(*****************)
+(* Substitutions *)
+(*****************)
+
+(* A substitution σ is a finite map from a variable x to a natural number i,
+   where σ[i]=x. 
+   This formulation of finite maps is unique because when a variable is removed from the list, 
+   all variables above that one are shifted downward. 
+*)
+Definition substitution := list Var.
+
+Print Gate_State.
+Record subst_state := Mk_subst_state
+  { get_σ : substitution
+  ; fresh : nat }. 
+
+Instance substitution_Gate_State : Gate_State subst_state :=
+  { get_fresh w st := let x := fresh st in 
+                      (x, Mk_subst_state (x :: get_σ st) (S x))
+  ; remove_var x st := let σ' := List.remove Nat.eq_dec x (get_σ st) in
+                        Mk_subst_state σ' (fresh st)
+  ; change_type x w st := st
+  }.
+                      
+
+Fixpoint mk_subst {w} (p : Pat w) : substitution :=
+  match p with
+  | unit       => []
+  | bit x      => [x]
+  | qubit x    => [x]
+  | pair p1 p2 => (mk_subst p1) ++ (mk_subst p2)
+  end.
+Definition mk_subst_state {w} (p : Pat w) : subst_state :=
+  let σ := mk_subst p in
+  Mk_subst_state σ (fold_left max σ 0).
+
+
+Definition remove_pat {A} `{Gate_State A} {w} (p : Pat w) (a : A) : A :=
+  fold_left (fun a x => remove_var x a)  (mk_subst p) a.
+
+
+(* Precondition: x must appear in li *)
+Fixpoint lookup (x : Var) (li : list Var) : nat :=
+  match li with
+  | nil => 0
+  | y :: ys => if x =? y then 0 else S (lookup x ys)
+  end.
+Fixpoint index {A} (i : nat) (li : list A) : option A :=
+  match i, li with
+  | _, nil => None
+  | 0, x :: _ => Some x
+  | S i', _ :: li' => index i' li'
+  end.
+
+Definition subst_var (σ : substitution) (x : Var) := lookup x σ.
+Fixpoint subst_pat (σ : subst_state) {w} (p : Pat w) : Pat w :=
+  match p with
+  | unit    => unit
+  | qubit x => qubit (subst_var (get_σ σ) x)
+  | bit   x => bit (subst_var (get_σ σ) x)
+  | pair p1 p2 => pair (subst_pat σ p1) (subst_pat σ p2)
+  end.
+
+Fixpoint subst_db (σ : subst_state) {w} (c : DeBruijn_Circuit w) 
+                : DeBruijn_Circuit w :=
+  match c with
+  | db_output p    => db_output (subst_pat σ p)
+  | db_gate g p c' => let p' := subst_pat σ p in
+                      let σ' := process_gate_state g p σ in
+                      db_gate g p' (subst_db σ' c')
+  | db_lift p f    => let p' := subst_pat σ p in
+                      let σ' := remove_pat p σ in
+                      db_lift p' (fun b => subst_db σ' (f b))
+  end.
+
+
+Print Gate_State.
+
+Definition Types_subst (Γ : DB_Ctx) (σ : substitution) (Γ' : DB_Ctx) :=
+  forall x x', lookup x σ = x' ->
+               (forall w, index x Γ = Some w <-> index x' Γ' = Some w).
+
+Lemma types_subst_length : forall Γ σ Γ',
+      Types_subst Γ σ Γ' -> length Γ = length Γ'.
+Proof.
+  induction Γ; intros σ Γ' pf.
+Admitted (* this will take some work, but it should be true *).
+
+  
+
+Lemma singleton_index : forall x w Γ,
+      SingletonCtx x w (DB_to_Ctx Γ) <-> ((index x Γ = Some w) * (length Γ = 1)).
+Proof.
+  induction x; intros.
+  - destruct Γ.
+    * split; simpl.
+      + inversion 1. 
+      + destruct 1 as [H _]; inversion H.
+    * split; simpl; intros H.
+      + inversion H; subst.
+        destruct Γ; [ | inversion H3].
+        split; auto.
+      + destruct H as [H1 H2].
+        inversion H1; subst.
+        destruct Γ; [ | inversion H2].
+        constructor.
+  - split; [intros H | intros [H1 H2]].
+    + inversion H. destruct Γ; inversion H1.
+    + destruct Γ; [inversion H2 | ]. 
+      simpl in *.
+      destruct Γ; [ | inversion H2].
+      destruct x; inversion H1.
+Qed.
+
+Lemma types_subst_pat_db : forall w (p : Pat w) Γ Γ' σ ,
+      Types_subst Γ (get_σ σ) Γ' ->
+      Types_DB_Pat Γ p ->
+      Types_DB_Pat Γ' (subst_pat σ p).
+Proof.
+  induction p; intros Γ Γ' σ types_σ types_p; simpl.
+  - assert (Γ = []) by (destruct Γ; auto; inversion types_p).
+    assert (eq_len : length Γ = length Γ') by (apply types_subst_length with (σ := get_σ σ); auto).
+    destruct Γ'; [ | subst; inversion eq_len].
+    constructor.
+  - unfold subst_var. inversion types_p. subst.
+    set (v' := lookup v (get_σ σ)).
+    set (eq_len := types_subst_length Γ (get_σ σ) Γ' types_σ).
+    set (types_σ' := types_σ v v' eq_refl Qubit).
+    set (singleton_index_pf := singleton_index v Qubit Γ).
+    assert (lookup_v' : index v' Γ' = Some Qubit).
+    { apply types_σ'. 
+      apply singleton_index_pf.
+      auto.
+    }
+    constructor.
+    apply singleton_index.
+    split.
+    + apply types_σ'.
+      apply singleton_index.
+      auto.
+    + replace 1 with (length Γ)
+        by (apply singleton_index_pf; auto).
+      apply eq_sym.
+      eapply types_subst_length; eauto.
+  - (* Same as above *)
+    unfold subst_var. inversion types_p. subst.
+    set (v' := lookup v (get_σ σ)).
+    set (eq_len := types_subst_length Γ (get_σ σ) Γ' types_σ).
+    set (types_σ' := types_σ v v' eq_refl Bit).
+    set (singleton_index_pf := singleton_index v Bit Γ).
+    assert (lookup_v' : index v' Γ' = Some Bit).
+    { apply types_σ'. 
+      apply singleton_index_pf.
+      auto.
+    }
+    constructor.
+    apply singleton_index.
+    split.
+    + apply types_σ'.
+      apply singleton_index.
+      auto.
+    + replace 1 with (length Γ)
+        by (apply singleton_index_pf; auto).
+      apply eq_sym.
+      eapply types_subst_length; eauto.
+  - unfold Types_DB_Pat.
+    (* requires an extra lemma here *)
+
+Admitted.
+
+  
+
+Lemma types_subst_db : forall w (c : DeBruijn_Circuit w) Γ ,
+      Types_DB Γ c ->
+      forall {σ Γ'},
+      Types_subst Γ (get_σ σ) Γ' ->
+      Types_DB Γ' (subst_db σ c).
+Proof.
+  induction 1; intros σ Γ' types_σ; simpl.
+  - constructor.
+    eapply types_subst_pat_db; eauto.
+  - econstructor; eauto.
+    * admit (* requires an extra lemma about merging and substituting *).
+    * eapply types_subst_pat_db; [ | eauto].
+      admit (* requires an extra lemma, possibly the same one as above *).
+    * apply IHTypes_DB.
+      admit (* requires another lemma... *).
+  - econstructor. admit. admit.
+    intros b. apply H2. admit.
+Admitted.
+    
+      
+             
+    
+
+
+(***************)
+(* composition *)
+(***************)
+Print subst_state.
+Fixpoint db_compose {w w'} (c : DeBruijn_Circuit w) (c' : DeBruijn_Circuit w') 
+                  : DeBruijn_Circuit w' :=
+  match c with
+  | db_output p   => subst_db (mk_subst_state p) c'
+  | db_gate g p c => db_gate g p (db_compose c c')
+  | db_lift p f   => db_lift p (fun b => db_compose (f b) c')
+  end.
+
+Lemma db_compose_correct : forall {w w'} (c : DeBruijn_Circuit w) (c' : DeBruijn_Circuit w') 
+                                  Γ1 Γ2 Γ,
+    Γ2 = WType_to_DB_Ctx w ->
+    Types_DB Γ1 c -> Types_DB (Γ2 ++ Γ) c' -> Types_DB (Γ1 ++ Γ) (db_compose c c').
